Velvet/Core.lean
@@ -8,8 +8,6 @@ public import Velvet.Core.Loop
 public import Velvet.Core.Partial
 public import Velvet.Core.VCGen
 public import Velvet.Core.NonDet
-public import Velvet.Core.Testing
-public meta import Velvet.Core.Testing
 
 open scoped GhostSyntax Std.WP Lean.Order
-open Std.WP Named Loop Specs WPPartial NonDetT Velvet.Testing
+open Std.WP Named Loop Specs WPPartial NonDetT
