Velvet/Core/Testing.lean
@@ -1,7 +1,0 @@
-module
-
-public import Velvet.Core.Testing.Decidable
-public meta import Velvet.Core.Testing.Decidable
-public import Velvet.Core.Testing.Gen
-
-open Velvet.Testing
