Velvet/Frontend.lean
@@ -9,5 +9,3 @@ public import Velvet.Frontend.Method
 public meta import Velvet.Frontend.Method
 public import Velvet.Frontend.ProveCorrect
 public meta import Velvet.Frontend.ProveCorrect
-public import Velvet.Frontend.Tester
-public meta import Velvet.Frontend.Tester
